Add work towards soundness theorems with constructor types

src/Soundness.v
@@ -10,15 +10,34 @@ Module Soundness (P : PAT).
     Module SmallStep := SmallStep M.
     Import Typing SmallStep.
 
+    Lemma tname_value_weakening :
+      forall G2 G1 ty t T,
+        T \notin tfv ty ->
+        is_value t ->
+        G1 & T ~ BindTName & G2 |= t ~: ty ->
+        G1 & G2 |= t ~: ty.
+    Admitted.
+
+    Lemma con_value_weakening :
+      forall G2 G1 ty t K d ty' T,
+        K \notin tfv ty ->
+        is_value t ->
+        G1 & K ~ BindCon d ty' T & G2 |= t ~: ty ->
+        G1 & G2 |= t ~: ty.
+    Admitted.
+
+    Definition no_vars (Gamma : env) : Prop :=
+      forall x ty, binds x (BindVar ty) Gamma -> False.
+
     Theorem progress :
-      forall t ty,
-        empty |= t ~: ty ->
+      forall Gamma t ty,
+        no_vars Gamma ->
+        Gamma |= t ~: ty ->
         is_value t \/ exists t', t --> t'.
     Proof.
-      introv hasType.
-      remember empty as Gamma.
+      introv Hnv hasType.
       induction hasType; substs*.
-      { Case "TmFVar". false. apply* binds_empty_inv. }
+      { Case "TmFVar". false. apply* Hnv. }
       { Case "TmApp". right.
         forwards* [Hval1 | (t1' & Hstep1)]: IHhasType1.
         forwards* [Hval2 | (t2' & Hstep2)]: IHhasType2.
@@ -28,9 +47,17 @@ Module Soundness (P : PAT).
         inverts Hval; inverts* hasType. }
       { Case "TmCon".
         forwards* [Hval | (t' & Hstep)]: IHhasType. }
-      { Case "TmType". admit. }
-      { Case "TmConDef". admit. }
-    Admitted.
+      { Case "TmType". right. pick_fresh T.
+        forwards* [Hval | (t' & Hstep)]: H1 T.
+        + introv Hb. binds_cases Hb. apply* Hnv.
+        + forwards* Hv : Topen_value Hval.
+        + forwards* (t'0 & Hstep') : Topen_step Hstep. }
+      { Case "TmConDef". right. pick_fresh K.
+        forwards* [Hval | (t' & Hstep)]: H4 K.
+        + introv Hb. binds_cases Hb. apply* Hnv.
+        + forwards* Hv : Kopen_value Hval.
+        + forwards* (t'0 & Hstep') : Kopen_step Hstep. }
+    Qed.
 
     Theorem preservation :
       forall Gamma t t' ty,
@@ -51,7 +78,21 @@ Module Soundness (P : PAT).
         rewrite* (@tsubst_intro X).
         rewrite* (@tsubst_t_intro X).
         apply_empty~ ok_term_tsubst. }
-    Admitted.
+      { Case "TmType". pick_fresh T.
+        assert (Htype : Gamma |= Topen_t 0 (FTName T) t' ~: ty).
+        { apply_empty* tname_value_weakening. auto. apply~ value_Topen. }
+        forwards~ Hnin : ok_term_notin T Htype.
+        forwards Heq : notin_Topen Hnin. rewrite~ Heq in Htype. }
+      { Case "TmTypeCong". apply_fresh TType as T ; auto.
+        forwards* Hstep': step_Topen t t2. }
+      { Case "TmConDef". pick_fresh K.
+        assert (Htype : Gamma |= Kopen_t 0 (FCon K) t' ~: ty2).
+        { apply_empty* con_value_weakening. auto. apply~ value_Kopen. }
+        forwards~ Hnin : ok_term_notin K Htype.
+        forwards Heq : notin_Kopen Hnin. rewrite~ Heq in Htype. }
+      { Case "TmConDefCong". apply_fresh TConDef as K; auto.
+        forwards* Hstep': step_Kopen t t2. }
+    Qed.
 
   End Soundness.
 End Soundness.
